---
title:  "Applied Electromagnetics For Engineers 01"
date:   2022-10-24 16:40:00 +0200
categories: analog-circuit
tags: tline
math: true
---

## Index

- [Lecture 01](#lecture-01)
- [Lecture 02 Circuit Model of Transmission Line](#lecture-02)
- [Lecture 03 Solution of Wave Equation](#lecture-03)
- [Lecture 04 Reflection Coefficient and Transmission Coefficient](#lecture-04)
- [Lecture 05 Circuit Parameters of a T-line](#lecture-05)

## Lecture 01

[Lecture 01 Youtube](https://www.youtube.com/watch?v=M_oYQ7zUbzA&list=PL2yOsdr0555KtDCv347wojVQ4wSb4KP3p&index=1)

## Lecture 02

[Lecture 02 Youtube](https://www.youtube.com/watch?v=surDm-x5Uwo&list=PL2yOsdr0555KtDCv347wojVQ4wSb4KP3p&index=2)

### Circuit Model of Transmission Line

- The model only include inductors on the one side.
- However the calculatoin result will be the same


![transmission line model](/assets/img/2022-10-24-applied-em-01/01.png)
_transmission line model_

Using KVL and KCL for the model

$$
\begin{align}
v(z) + L \Delta z \frac{\partial i(z,t)}{\partial t} + v(z+\Delta z) &= 0\\
i(z) - i(z+\Delta z) - C \Delta z \frac{\partial v(z+\Delta z)}{\partial t} &= 0
\end{align}
$$

that is

$$
\begin{align}
\frac{\partial v(z,t)}{\partial z} &= -L \frac{\partial i(z,t)}{\partial t}\\
\frac{\partial i(z,t)}{\partial z} &= -C \frac{\partial v(z,t)}{\partial t}
\end{align}
$$

that is

$$
\begin{align}
\frac{\partial^2 v}{\partial z^2} &= LC \frac{\partial^2 v}{\partial t^2}\\
\frac{\partial^2 i}{\partial z^2} &= LC \frac{\partial^2 i}{\partial t^2}
\end{align}
$$

## Lecture 03

[Lecture 03 Youtube](https://www.youtube.com/watch?v=izGLJ2Lknn0&list=PL2yOsdr0555KtDCv347wojVQ4wSb4KP3p&index=4)

### Solution of Wave Equation

For the wave equation like the form

$$
\begin{align}
\frac{\partial^2 v}{\partial z^2} &= LC \frac{\partial^2 v}{\partial t^2}
\end{align}
$$

the solution is $$v(t,z) = f(t - \sqrt{LC} z)$$ or $$v(t,z) = f(t + \sqrt{LC} z)$$ with reasonable $$f(.)$$

if

$$
v(t,z) = f(t-\sqrt{LC}z)
$$

then the wave is travelling to the positive direction of $$z$$, with phase velocity

$$
\mu_{p} = \dfrac{\Delta z}{\Delta t} = \dfrac{1}{\sqrt{LC}}
$$

e.g.,

$$
v(t,z) = \cos(\omega t - \beta z)
$$

where

$$
\dfrac{\omega}{\beta} = \dfrac{1}{\sqrt{LC}}
$$

### Phasor Representation

If we assume all the signal have the same angular frequency $$\omega$$, we can represent the signal by phasor. e.g., if the wave is transmited to the positive side of $$z$$ axis,

$$
\begin{align}
V(z) &= V_0^{+} e^{-j\beta z}\\
I(z) &= I_0^{+} e^{-j\beta z}
\end{align}
$$

is the phasor representation of $v(z,t) = V_0^{+}\cos(\omega t - \beta z)$, and $$i(z,t) = I_0^{+}\cos(\omega t - \beta z)$$

using equation

$$
\begin{align}
\frac{\partial v(z,t)}{\partial z} &= -L \frac{\partial i(z,t)}{\partial t}\\
\end{align}
$$

we can get

$$
\begin{align}
I_0^+ &= \dfrac{V_0^+}{Z_0}\\
Z_0 &= \sqrt{\frac{L}{C}}
\end{align}
$$

the $$\sqrt{L/C}$$ is called characteristic impedance of the transmission line.


## Lecture 04

[Lecture 04 Youtube](https://www.youtube.com/watch?v=n7zqIsI7lZ8&list=PL2yOsdr0555KtDCv347wojVQ4wSb4KP3p&index=4)

### Reflection Coefficient

assume the wave is the superposition of two directions

$$
\begin{align}
\widetilde{V}(z) &= V_0^+ e^{-j\beta z} + V_0^- e^{j \beta z}
\end{align}
$$

then using equation

$$
\begin{align}
\frac{\partial v(z,t)}{\partial z} &= -L \frac{\partial i(z,t)}{\partial t}\\
\end{align}
$$

we can get

$$
\begin{align}
\widetilde{I}(z) &= I_0^{+} e^{-j\beta z} + I_0^{-} e^{j\beta z}\\
&= \dfrac{V_{0}^+}{Z_0} e^{-j\beta z} - \dfrac{V_0^-}{Z_0} e^{j\beta z}
\end{align}
$$

now assume we put a load $$Z_L$$ at $$z=0$$ (the wave is coming from negative infinity size)

$$
\begin{align}
\widetilde{V}(z=0) &= V_0^{+} + V_0^- = V_L\\
\widetilde{I}(z=0) &= \dfrac{V_0^+}{Z_0} - \dfrac{V_0^-}{Z_0} = I_L\\
Z_L &= \dfrac{V_L}{I_L}
\end{align}
$$

from the equations we can get load reflection coefficient $$\Gamma_L$$

$$
\Gamma_L = \dfrac{V_0^-}{V_0^+} = \dfrac{Z_L-Z_0}{Z_L+Z_0}
$$

- if $$Z_L = \infty$$ (the T-line is terminated by open circuit)

$$
\Gamma_L = 1
$$

and

$$
\begin{align}
\widetilde{V}(z) &= V_0^+ (e^{-j\beta z} + e^{j\beta z}) = 2 V_0^+ \cos\beta z\\
v(z,t) &= 2 V_0^+ \cos\beta z\cdot \cos\omega t
\end{align}
$$

the above is a standing wave.

- if $$Z_L = 0$$ (the T-line is terminated by short circuit)

$$
\Gamma_L = -1
$$

and

$$
\begin{align}
\widetilde{V}(z) &= V_0^+(e^{-j\beta z} - e^{j\beta z}) = -2jV_0^+ \sin \beta z
\end{align}
$$

- if $$Z_L = Z_0$$

$$\Gamma_L = 0$$


$$
\begin{align}
\widetilde{V}(z) &= V_0^+ e^{-j\beta z}\\
v(z,t) &= V_0^+ \cos(\omega t - \beta t)
\end{align}
$$

### Transmission Coefficient


![transmissiom coefficient model](/assets/img/2022-10-24-applied-em-01/02.png)
_transmission coefficient model_

In the model we didn't consider the reflected wave after $$Z_L$$, since we assume the next load is at infinty, thus it will take very long time to reflect back.
We already made calculation for $$V_i^+$$ and $$V_r^-$$ if there is a $$Z_L$$. Now we want to determine $$V_t^+$$.

$$
\begin{align}
V_i^+(z=0) + V_r^-(z=0) &= V_L = V_t^+(z=0)\\
\dfrac{V_i^+(z=0)}{Z_{01}} - \dfrac{V_r^-(z=0)}{Z_{01}} &= I_L + \dfrac{V_t^+(z=0)}{Z_{02}}
\end{align}
$$

you can get reflection coefficient

$$
\begin{align}
\dfrac{V_r^+(z=0)}{V_i^+(z=0)} &= \Gamma_L = \dfrac{Z_{L\Vert} - Z_{01}}{Z_{L\Vert} + Z_{01}}
\end{align}
$$

where

$$
Z_{L\Vert} = \dfrac{Z_L Z_{02}}{Z_L + Z_{02}} = Z_L \Vert Z_{02}
$$

and transmission coefficient

$$
\tau = \dfrac{V_t^+(z=0)}{V_i^+(z=0)} = \dfrac{2Z_{L\Vert}}{Z_{L\Vert} + Z_{01}}
$$

## Lecture 05

[Lecture 05 Youtube](https://www.youtube.com/watch?v=7xqTBXlpwFQ&list=PL2yOsdr0555KtDCv347wojVQ4wSb4KP3p&index=5)

### A Paradox Example

Assume a ideal voltage source (at $$z=-l$$) with voltage $$V_s \cos \omega t$$ to drive a lossless T-line.
The other end (at $$z=0$$) is terminated by a scope (with infity impedance).

For the open circuit termination, reflection coefficient is 1, and

$$
\begin{align}
\widetilde{V}_{line}(z) &= 2 V_0^+ \cos \beta z
\end{align}
$$

thus at $$z = 0$$

$$
v(t) = 2 V_0^+ \cos\omega t
$$

at $$z = -l$$

$$
v(t) = 2 V_0^+ \cos \beta l \cdot \cos \omega t = V_s \cos \omega t
$$

thus

$$
\begin{align}
2V_0^+ &= V_s / \cos\beta l
\end{align}
$$

then by choosing some $$l$$, e.g., $$\beta l=\pi/2$$ ,you can get infinity amplified voltage at the scope.

### Real Voltage Source

Ideal voltage source doesn't exist (otherwise it can provide infinity power to drive a short circuit load).

Now we assume the voltage source $$\widetilde{V}_{s}$$ is followed by impedance $$Z_s$$.
And the load is modeled by $$Z_L$$.

$$
\widetilde{V}_s = \widetilde{I}_{line}(-l) \cdot Z_s + \widetilde{V}_{line}(-l)
$$

if we assume $$Z_s = \infty$$ (open circuit), we know $$\Gamma_L = 1$$, and

$$
\begin{align}
V_0^+ &= V_0^-\\
\widetilde{V}_{line}(z) &= 2 V_0^+ \cos \beta z\\
\widetilde{I}_{line}(z) &= \dfrac{V_0^+}{Z_0} e^{-j\beta z} - \dfrac{V_0^-}{Z_0} e^{j\beta z}\\
&= \dfrac{V_0^+}{Z_0} e^{-j\beta z} - \dfrac{V_0^+}{Z_0} e^{j\beta z}
\end{align}
$$

if we assume $$\beta l = \pi/2$$

$$
\widetilde{V}_s = 2 j \dfrac{V_0^+}{Z_0} \cdot Z_s
$$

and

$$
V_0^+ = -j\dfrac{Z_0}{2Z_s} \widetilde{V}_s
$$

### Line Impedance and Input Impedance

we know

$$
\begin{align}
\widetilde{V}_{line}(z) &= V_0^+ e^{-j\beta z} + V_0^- e^{j\beta z}\\
\widetilde{I}_{line}(z) &= \dfrac{V_0^+}{Z_0} e^{-j \beta z} - \dfrac{V_0^-}{Z_0} e^{j \beta z}
\end{align}
$$

define line impedance (note the difference between line impedance and characteristic impedance)


$$
\begin{align}
Z_{line}(z) &= \dfrac{\widetilde{V}_{line}(z)}{\widetilde{I}_{line}(z)}\\
&= \dfrac{V_0^+ e^{-j\beta z} + V_0^- e^{j\beta z}}{\dfrac{V_0^+}{Z_0} e^{-j \beta z} - \dfrac{V_0^-}{Z_0} e^{j \beta z}}
\end{align}
$$

thus we can find the input impedance

$$
Z_{in} = Z_{line}(-l)
$$

using

$$
\begin{align}
V_0^- &= \Gamma_L V_0^+\\
\Gamma_L &= \dfrac{Z_L - Z_0}{Z_L + Z_0}
\end{align}
$$

we have

$$
\begin{align}
Z_{in} &= Z_0 \Bigg( \dfrac{Z_L \cos \beta l + j Z_0 \sin \beta l}{Z_0 \cos \beta l + j Z_L \sin \beta l} \Bigg)\\
&= Z_0 \Bigg( \dfrac{Z_L + j Z_0 \tan \beta l}{Z_0 + j Z_L \tan \beta l} \Bigg)
\end{align}
$$

we call $$\beta l$$ as electrical length.

### Example

A voltage source $$V_s = 10 \cos (\omega t + \pi/6)$$, or phasor $$10 \cdot e^{j \pi/6}$$
