---
title:  "Trigonometry"
date:   2022-10-10 12:00:00 +0200
categories: math
tags: basics
math: true
---

$$

\begin{align*}
    \cot \theta &= \frac{1}{\tan\theta}\\
    \sec \theta &= \frac{1}{\cos\theta}\\
    \csc \theta &= \frac{1}{\sin\theta}\\
    \frac{e^{i\theta} + e^{-i\theta}}{2} &= \cos\theta\\
    \frac{e^{i\theta} - e^{-i\theta}}{2i} &= \sin\theta\\
    sinc(x) &= \frac{\sin(\pi x)}{ \pi x}\\
    \sin(\alpha + \beta) &= \sin\alpha\cos\beta + \cos\alpha\sin\beta\\
    \sin(\alpha - \beta) &= \sin\alpha \cos\beta - \cos\alpha \sin \beta\\
    \cos(\alpha + \beta) &= \cos\alpha \cos\beta - \sin\alpha \sin\beta\\
    \cos(\alpha - \beta) &= \cos\alpha\cos\beta + \sin\alpha \sin\beta\\
    \sin \alpha \cos \beta &= \frac{1}{2}\big( \sin(\alpha + \beta) + \sin(\alpha -\beta) \big)\\
    \cos\alpha \sin\beta &= \frac{1}{2}\big( \sin(\alpha + \beta) - \sin(\alpha - \beta) \big)\\
    \cos\alpha \cos\beta &= \frac{1}{2}\big( \cos(\alpha + \beta) + \cos(\alpha - \beta) \big)\\
    \sin\alpha \sin\beta &= -\frac{1}{2}\big( \cos(\alpha + \beta) - \cos(\alpha - \beta) \big)\\
    A\sin\alpha + B\cos\alpha &= \sin(\alpha+\varphi)\quad\textrm{where }\tan\varphi = \frac{B}{A}\\
    A\sin\alpha - B\cos\alpha &= \sin(\alpha - \varphi)\quad\textrm{where }\tan\varphi = \frac{B}{A}\\
    A\cos\alpha - B\sin\alpha &= \cos(\alpha + \varphi)\quad\textrm{where }\tan\varphi = \frac{B}{A}\\
    A\cos\alpha + B\sin\alpha &= \cos(\alpha - \varphi)\quad\textrm{where }\tan\varphi = \frac{B}{A}\\
    \sin^2\theta &= \frac{1 - \cos(2\theta)}{2}\\
    \cos^2(\theta) &= \frac{1 + \cos(2\theta)}{2}\\
    \cos^3(\theta) &= \frac{3}{4}\cos\theta + \frac{1}{4}\cos 3\theta\\
    \mathrm{E}[\sin^2(t)] &= \frac{1}{2}\\
\end{align*}
$$
