---
title:  "Calculus 005"
date:   2023-05-27 07:00:00 +0200
categories: math
tags: math
math: true
---

From [Zhenyu Qi' Lecture 005](http://ocw.aca.ntu.edu.tw/ntu-ocw/ocw/cou/104S115/5)

## Series Convergent Criterion

$$
\sum_{n} a_n \text{ converges} \iff s_{n} (n \in \mathbb{N}) \text{ converges } \iff s_n (n \in \mathbb{N}) \text{ is Cauchy}
$$

$$
\forall \varepsilon > 0, \exists N \in \mathbb{N}, [k > N, l \ge 0 \implies \vert a_k + \dots + a_{k+l} \vert < \varepsilon ]
$$

since

$$
\vert a_{k} + \dots + a_{k+l} \vert \le \vert a_k \vert + \dots + \vert a_{k+l} \vert
$$

thus if we have $$ \sum_n \vert a_n \vert$$ convergent, we are sure $$\sum_{n} a_n$$ convergent.
Since the partial sum of $$\sum_{n} \vert a_n \vert$$ monotone, it converges if and only if its partial sum has a upper bound.

$$
\exists M > 0 \forall n \in \mathbb{N} [\vert a_1 \vert + \dots \vert a_n \vert \le M]
$$

Notation: If $$a_n \ge 0 (n \in \mathbb{N})$$, then we write $$\sum_{n} a_n < \infty$$ to mean that $$\sum_n a_n$$ converges.
We write $$\sum_{n} a_n = \infty$$ to mean that it diverges.

Examples (1) $$\sum_{n=1}^{\infty} \frac{1}{n}$$

$$
S_1 = 1
$$

$$S_2 = 1 + \frac{1}{2}$$

$$
S_4 = 1 + \frac{1}{2} + \frac{1}{3} + \frac{1}{4} > 1 + \frac{1}{2} + \frac{1}{2}
$$

$$
\begin{align}
\forall m \in \mathbb{N}, S_{2^m} &= 1 + \frac{1}{2} + \frac{1}{3} + \frac{1}{4} + \dots + \frac{1}{2^{m-1}+1} + \dots + \frac{1}{2^{m-1}+2^{m-1}}\\
& > 1 + \frac{m}{2}
\end{align}
$$

(2) $$\sum_{n=1}^{\infty} \frac{1}{n^2}$$

$$
\frac{1}{n^2} < \frac{1}{n(n-1)} = \frac{1}{n-1} - \frac{1}{n}
$$

$$
\begin{align}
S_n &= 1 + \frac{1}{2^2} + \dots + \frac{1}{n^2} < 1 + (\frac{1}{1} - \frac{1}{2}) + (\frac{1}{2}-\frac{1}{3}) + \dots + (\frac{1}{n-1} - \frac{1}{n})\\
& < 1 + 1 - \frac{1}{n} < 2
\end{align}
$$

(3) $$\sum_{n=1}^{\infty} \dfrac{\sin(n)}{n^k}$$, for $$k \in \mathbb{N}, k \ge 2$$

$$
\vert \dfrac{\sin(1)}{1^k} \vert + \dots + \vert \dfrac{\sin(n)}{n^k} \vert < 1 + \dots + \frac{1}{n^2} < 2
$$

thus $$\sum_{n=1}^{\infty} \dfrac{\sin(n)}{n^k}$$ converges.

Ex2. For $$a > 1$$ and $$k \in \mathbb{N}$$, show that $$\sum_{n=1}^{\infty} \frac{n^k}{a^n} < \infty$$

It is obvious all terms are non-negative.
Similar from the exercise in Calculus 003, for any $$n > 2k+ 4 > k+2$$

$$a^n = (1+b)^n \ge \binom{n}{k+2} b^{k+2} \ge \dfrac{b^{k+2}}{(k+2)!}(n-k-1)^{k+2} \ge \dfrac{b^{k+2}}{2^{k+2}(k+2)!} n^{k+2}$$

thus for any $$n > 2k + 4$$

$$
\dfrac{n^k}{a^n} \le \dfrac{2^{k+2}(k+2)!}{b^{k+2}} \dfrac{1}{n^2}
$$

thus the partial sum has upper bound.

Def: Given a sequence $$a_n (n \in \mathbb{N})$$, we say that

(1) $$\sum_{n} a_n$$ converges absolutely if $$\sum_{n} \vert a_n \vert < \infty$$.

(2) $$\sum_{n} a_n$$ converges conditionally if $$\sum_{n} \vert a_n \vert = \infty$$ but $$\sum_{n=1}^{\infty} a_n$$ converges.

## Comparison Test

If $$a_n, b_n (n \in \mathbb{N}) \ge 0$$

(1) If we have

$$\exists C > 0 \text{ and } N \in \mathbb{N} [n \ge N \implies a_n \le C b_n]$$

then

$$
\sum_n b_n < \infty \implies \sum_n a_n < \infty
$$

Proof:

Since they are non-negative series, their convergence are equivalent to that the partial sum has upper bound.
From the partial sum of $$b_n$$ has upper bound, it is obvious that the partial sum of $$a_n$$ has upper bound.

(2) If we know

$$
\lim_{n\to\infty} \dfrac{a_n}{b_n} \text{ exists }
$$

then

$$\exists C > 0 \text{ and } N \in \mathbb{N} [n \ge N \implies a_n \le C b_n]$$

Proof:

Let $$l = \lim_{n\to\infty} \dfrac{a_n}{b_n}$$ and $$\varepsilon=1$$

$$
\exists N \in \mathbb{N} [n \ge N \implies l-1 < \dfrac{a_n}{b_n} < l+1]
$$

$$
\exists N \in \mathbb{N} [n \ge N \implies a_n < (l+1)b_n]
$$

where $$l+1$$ must be positive $$(C > 0)$$, since $$l \ge 0$$.

If $$\lim_{n\to\infty} \dfrac{a_n}{b_n}$$ exists and not equal $$0$$, it is easy to see $$\sum_{n} a_n < \infty \iff \sum_{n} b_n < \infty$$, since $$a_n, b_n$$ can be bounded by each other.

- Actually, $$\lim_{n\to\infty} \dfrac{a_n}{b_n}$$ exists can be replaced by $$\overline{\lim_{n\to\infty}} \dfrac{a_n}{b_n}$$ exists.

Proof: Let $$u_n = \sup \{\dfrac{a_m}{b_m} \vert m \ge n\}$$, $$\lim_{n\to\infty}u_n = l$$.

$$
\exists N \in \mathbb{N} [u_N < l+1]
$$

$$
\exists N \in \mathbb{N} [l+1 \text{ is an upper bound of } \{\dfrac{a_m}{b_m} \vert m \ge N\}]
$$

$$
\exists N \in \mathbb{N} [n \ge N \implies \dfrac{a_n}{b_n} \le l + 1]
$$

## Ratio and Root Tests

Exercise 3 (the ratio and the root tests):

Let $$a_n (n \in \mathbb{N}) \ge 0$$. Then

(1) If $$\lim_{n\to\infty} \dfrac{a_{n+1}}{a_n} < 1$$, then

$$
\exists N \in \mathbb{N} \text{ and } C < 1 [n \ge N \implies a_{n+1} \le C a_n]
$$

then, $$\sum_{n} a_n < \infty$$

Proof: the idea is that

$$
\exists N \in \mathbb{N} \text{ and }0 < C < 1 [n \ge N \implies a_{n} \le C^{n-N} a_N]
$$

Since the series $${a_1, a_2, \dots, a_{N-1}, C^{0} a_{N}, C^{1} a_{N}, \dots}$$ converges, we know $$a_n (n\in\mathbb{N})$$ converges.

Similarly, if $$\lim_{n\to\infty} \dfrac{a_{n+1}}{a_n} > 1$$, we have $$\sum_n a_n = \infty$$.

If $$\lim_{n\to\infty} \dfrac{a_{n+1}}{a_n} = 1$$, it may converge or diverge.

(2) If $$\lim_{n\to\infty} (a_n)^{1/n} < 1$$, then

$$
\exists N \in \mathbb{N} \text{ and } C < 1 [n \ge N \implies a_n \le C^n]
$$

thus $$\sum_{n} a_n < \infty$$.

If $$\lim_{n\to\infty} (a_n)^{1/n} > 1$$, then $$\sum_{n} a_n = \infty$$.

## Alternating Series

Question: does $$\sum_{n=1}^{\infty} \dfrac{(-1)^{n-1}}{n}$$ converges (conditionally)?

Def: A series $$\sum_n a_n$$ is an alternating series if

$$
\exists b_n > 0 (n \in \mathbb{N}) \text{ s.t. } a_n = (-1)^{n-1} b_n (n \in \mathbb{N})
$$

Confusion: $$b_n > 0$$ or $$b_n \ge 0$$?

## Leibniz's Criterion

If $$\sum_n a_n$$ is an alternating series, and $$b_n (=\vert a_n \vert) \searrow 0$$ as $$n \to \infty$$ (monotonically non-increasing, and converges to $$0$$), then $$\sum_{n} a_n$$ converges.

Proof:

We know $$b_n = (-1)^{n-1} a_n$$. Consider the tail

$$
\vert a_k + \dots + a_{k+l} \vert = \vert (-1)^{k-1} (b_k - b_{k+1} + \dots + (-1)^l b_{k+l}) \vert
$$

It is easy to see that $$b_k - b_{k+1} + \dots + (-1)^{l} b_{k+l} \ge 0$$, no matter $$l$$ is even or odd.

$$
\begin{align}
&\vert a_k + \dots + a_{k+l} \vert = \vert (-1)^{k-1} (b_k - b_{k+1} + \dots + (-1)^l b_{k+l}) \vert\\
=& b_k - b_{k+1} + \dots + (-1)^l b_{k+l} \le b_k
\end{align}
$$

It is smaller than $$b_k$$ since you can calculate it as $$b_k - (b_{k+1}-b_{k+2}) - \dots$$, no matter $$l$$ is even or odd.

Plus we know $$\lim_{n\to\infty} b_n = 0$$, the tail can be controlled, and the series $$\sum_{n} a_n$$ converges.
