---
title:  "Noise Bandwidth"
date:   2023-03-20 07:00:00 +0200
categories: math
tags: math
math: true
---

$$
 H(s) = \dfrac{1}{1 + \dfrac{s}{\omega_0 Q} + \dfrac{s^2}{\omega_0^2}}
$$

$$
H(j\omega) = \dfrac{1}{1 + \dfrac{j\omega}{\omega_0 Q} + \dfrac{(j\omega)^2}{\omega_0^2}}
$$

$$
H(-j\omega) = \dfrac{1}{1 - \dfrac{j\omega}{\omega_0 Q} + \dfrac{(-jω)^2}{\omega_0^2}}
$$

$$
\vert H(j\omega)\vert^2 = H(j\omega)H(-j\omega) = \dfrac{1}{(1 + \dfrac{jω}{\omega_0 Q} + \dfrac{(jω)^2}{\omega_0^2})(1 - \frac{jω}{\omega_0 Q} + \frac{(-jω)^2}{\omega_0^2})}
$$
