---
title:  "Calculus 006"
date:   2023-05-29 07:00:00 +0200
categories: math
tags: math
math: true
---

From [Zhenyu Qi' Lecture 006](http://ocw.aca.ntu.edu.tw/ntu-ocw/ocw/cou/104S115/6)

## Seperated Sequences

Given a sequence $$a_n (n \in \mathbb{N})$$, we can seperate all terms into two sequences:

$$
a_{n_1}, a_{n_2}, \dots \text{ and } a_{n_1'}, a_{n_2'}, \dots
$$

with

$$
n_1 < n_2 < \dots \text{ and } n_1' < n_2' < \dots
$$

also

$$
\begin{align}
\{n_1, n_2, \dots\} \cup \{n_1', n_2', \dots\} &= \mathbb{N}\\
\{n_1, n_2, \dots\} \cap \{n_1', n_2', \dots\} &= \emptyset
\end{align}
$$

s.t. $$a_{n_j} \ge 0 (j \in \mathbb{N})$$ and $$a_{n_k'} \le 0 (k \in \mathbb{N})$$

Let $$p_j := a_{n_j} (j \in \mathbb{N})$$ and $$q_k := - a_{n_k'} (k \in \mathbb{N})$$, we know $$p_j \ge 0, q_k \ge 0$$.

Exercise 3: Show that

$$
\sum_{n} \vert a_n \vert < \infty \iff \sum_{j} p_j < \infty \land \sum_{k} q_k < \infty
$$

Moreover, if and side holds, then

$$
\sum_{n} \vert a_n \vert = \sum_{j} p_j + \sum_k q_k $$

$$ \sum_{n} a_n = \sum_{j} p_j - \sum_k q_k
$$

Proof:

&nbsp; $$\implies$$: Let the partial sum of $$\sum_n \vert a_n \vert$$ has upper bound M.

The partial sum of $$\sum_j p_j$$ is less or equal to the partial sum of $$\sum_n \vert a_n \vert$$

$$
\begin{align}
&p_1 + \dots + p_k = a_{n_1} + \dots + a_{n_k}\\
\le & \vert a_1 \vert + \vert a_2 \vert + \dots + \vert a_{n_k} \vert \le M
\end{align}
$$

Thus the right side has upper bound, thus converges.

&nbsp; $$\Longleftarrow$$: Let the partial sum of $$\sum_j p_j, \sum_k q_k$$ has uppber bound $$U, V$$ respectively. Consider the partial sum of $$\sum_n \vert a_n \vert$$

$$
\vert a_1 \vert + \dots + \vert a_k \vert \le p_1 + \dots + p_k + q_1 + \dots + q_k \le U + V
$$

To prove $$\sum_{n} \vert a_n \vert = \sum_{j} p_j + \sum_k q_k$$, let $$s_k = \vert a_1 \vert + \dots + \vert a_k \vert$$, $$u_k = p_1 + \dots + p_k$$, $$v_k = q_1 + \dots + q_k$$, and let

$$
\lim_{k\to \infty} u_k = L_p
$$

$$
\lim_{k\to\infty} v_k = L_q
$$

We know

$$
s_k \le u_k + v_k \implies \lim_{k \to \infty} s_k \le L_p + L_q
$$

also

$$
u_k + v_k \le s_{\max(n_k, n'_k)}
$$

It is easy to see $$\lim_{k\to\infty} s_{\max(n_k,n'_k)} = \lim_{k\to\infty} s_k$$, thus

$$
\lim_{k\to\infty} s_k \ge L_p + L_q
$$

Thus $$\sum_{n} \vert a_n \vert = \sum_{j} p_j + \sum_k q_k$$.

To prove $$\sum_{n} a_n = \sum_j p_j - \sum_k q_k$$, now let $$s_k = a_1 + \dots + a_k$$

$$
\forall \varepsilon > 0 \exists N \in \mathbb{N} [k \ge N \implies \vert u_k - L_p \vert < \varepsilon \land \vert v_k - L_q \vert < \varepsilon]
$$

$$
k \ge \max(n_N, n_N') \implies s_{k} = u_{N_1} - v_{N_2}, \text{ where } N_1 \ge N, n_2 \ge N
$$


$$
 k \ge \max(n_N, n_N') \implies \vert s_{k} - (L_p - L_q) \vert = \vert (u_{N_1} - L_p) + (v_{N_2} - L_q) \vert \le 2 \varepsilon
$$

Thus $$\sum_{n} a_n = \sum_j p_j - \sum_k q_k$$.

## Two Convergent Series

- &nbsp; $$\sum_n a_n$$ and $$\sum_n b_n$$ converge $$\implies \sum_{n} (a_n \pm b_n) = \sum_n a_n \pm \sum_n b_n$$

$$
A_n = a_1 + \dots + a_n, B_n = b_1 + \dots + b_n, S_n = a_1 + b_1 + \dots + a_n + b_n
$$

$$
\forall \varepsilon > 0 \exists N \in \mathbb{N} [n \ge N \implies \vert A_n - A \vert < \varepsilon \land \vert B_n - B \vert < \varepsilon]
$$

$$
\forall \varepsilon > 0 \exists N \in \mathbb{N} [n \ge N \implies \vert S_n - (A + B)\vert < 2 \varepsilon]
$$

- Inserting finite number of 0s into all the two neighbor terms, will not affect its convergence or divergence and its sum (if the sum exists).

16min
