---
title:  "Calculus 003"
date:   2023-05-18 07:00:00 +0200
categories: math
tags: math
math: true
---

From [Zhenyu Qi' Lecture 003](http://ocw.aca.ntu.edu.tw/ntu-ocw/ocw/cou/104S115/3)

Example: If $$a>1$$, then $$\lim_{n\to\infty} \dfrac{1}{a^n} = 0$$.

$$
\dfrac{1}{(1+(a-1))^n} = \dfrac{1}{(1+b)^n} \le \dfrac{1}{1 + nb}
$$


Ex1 (squeeze theorem): $$\lim_{n\to\infty}a_n = \lim_{n\to\infty}b_n = L$$, and $$a_n \le c_n \le b_n$$, then $$\lim_{n\to\infty}c_n = L$$.

$$\forall \varepsilon > 0, \exists N_a, N_b \in \mathbb{N} [n \ge \max(N_a, N_b) \implies L-\epsilon < a_n \le b_n < L + \epsilon]$$

$$\forall \varepsilon > 0, \exists N_a, N_b \in \mathbb{N} [n \ge \max(N_a, N_b) \implies L-\epsilon < a_n \le c_n \le b_n < L + \epsilon]$$


Ex: prove for any $$k \in \mathbb{N}$$, and real number $$a > 1$$, $$\lim_{n\to\infty} \dfrac{n^k}{a^n} = 0$$

Let $$a = 1+b$$ where $$b > 0$$.

$$
\text{ for any } n > k+1, \quad a^n = (1+b)^n \ge \binom{n}{k+1}b^{k+1} \ge \dfrac{b^{k+1}}{(k+1)!} (n-k)^{k+1}
$$

$$
0 \le \dfrac{n^k}{a^n} \le \dfrac{n^k}{(n-k)^k} \dfrac{1}{n-k} \dfrac{k!}{b^k}
$$

By squeeze theorem, we have $$\lim_{n\to\infty} \dfrac{n^k}{a^n} = 0$$.

## Monotone

(1) nondecreasingly monotone / increasing: $$\forall n \in N, a_n \le a_{n+1}$$

nonincreasingly monotone / decreasing: $$\forall n \in N, a_n \ge a_{n+1}$$

$$
a_n \nearrow \quad a_n \searrow
$$

(2) strictly increasing (resp. strictly decreasing)

$$
a_n \nearrow\nearrow \quad a_n \searrow\searrow
$$

Theorem: (boundedness from above $$+ \nearrow \implies $$ convergence)

Since it is boundedness from above, let $$L = \sup \{a_n\}$$.

$$
\forall \varepsilon> 0, L - \varepsilon \text{ is not upper bound}, \exists N \in \mathbb{N}, [n \ge N \implies a_n \ge a_{N} > L - \varepsilon]
$$

plus $$a_n \le L$$, we have $$\vert a_n - L \vert < \epsilon$$.

## The Decimal Expression

Examples: (1) A decimal expression gives a real number.

$$0.d_1 d_2 d_3 \dots$$

$$
a_1 = 0.d_1, a_2 = 0.d_1 d_2, \dots
$$

$$
\forall n \in \mathbb{N} \, [a_n \in \mathbb{Q}]
$$

$$
a_n \nearrow, \text{ it has uppber bound } 1
$$

one real number may have different decimal expression, 1, 0.999999

## The Natural Base

(2) The natural base $$e$$

$$
e = \lim_{n\to\infty} (1 + \dfrac{1}{n})^n
$$

$$
\begin{align}
a_n &= \binom{n}{0} + \binom{n}{1}\dfrac{1}{n} + \binom{n}{2}\dfrac{1}{n^2} + \dots + \binom{n}{n}\dfrac{1}{n^n}\\
&= \sum_{j=0}^n \binom{n}{j}\dfrac{1}{n^j}
\end{align}
$$

$$
\binom{n}{j} = \dfrac{n!}{j!(n-j)!}
$$

$$
\begin{align}
&\dfrac{n!}{j!(n-j)!} \dfrac{1}{n^j} = \dfrac{1}{j!} \dfrac{n (n-1) \dots (n-j+1)}{n^j}\\
=& \dfrac{1}{j!} (1-\frac{1}{n})(1-\frac{2}{n})\dots (1 - \dfrac{j-1}{n})
\end{align}
$$

$$
a_n = 1 + 1 + \dfrac{1}{2!}(1-\frac{1}{n}) + \dfrac{1}{3!}(1-\frac{1}{n})(1-\frac{2}{n}) + \dots + \dfrac{1}{n!}(1-\frac{1}{n})\dots (1-\frac{n-1}{n})
$$

$$
a_{n+1} = 1 + 1 + \dfrac{1}{2!}(1-\frac{1}{n+1}) + \dfrac{1}{3!}(1-\frac{1}{n+1})(1-\frac{2}{n+1}) + \dots + \dfrac{1}{n!}(1-\frac{1}{n+1})\dots (1-\frac{n-1}{n+1}) + \dfrac{1}{(n+1)!}(1-\frac{1}{n+1})\dots (1-\frac{n}{n+1})
$$

thus

$$
a_{n+1} > a_{n} \quad a_{n} \nearrow\nearrow
$$

and

$$
\begin{align}
a_n &< 1 + 1 + \frac{1}{2!} + \dots + \frac{1}{n!}\\
&< 1 + 1 + \frac{1}{2} + \frac{1}{2^2} + \dots \frac{1}{2^{n-1}}\\
&= 1 + \dfrac{1-\frac{1}{2^n}}{1-\frac{1}{2}} < 3
\end{align}
$$

in the near future we will see that

$$
e = \lim_{n\to\infty}(1 + 1 + \frac{1}{2!} + \dots + \frac{1}{n!})
$$

## Nested Intervals

Definition: A sequence of intervals $$I_n (n \in \mathbb{N})$$ is nested if $$I_n \ne \emptyset$$ and $$I_{n+1} \subseteq I_n$$ for all $$n \in \mathbb{N}$$.

Question: $$\bigcap\limits_{n\in\mathbb{N}} I_n \ne \emptyset$$?

Sometimes it becomes emptyset.

(1) $$I_n = (0, \frac{1}{n})$$

(2) $$I_n = [n, \infty)$$

Theorem (of nested intervals)

If $$I_{n} (n \in \mathbb{N})$$ is a sequence of bounded closed nested intervals ($$[a_n, b_n]$$), then $$\bigcap\limits_{n\in\mathbb{N}}I_n \ne \emptyset$$.

Proof:

Write $$I_n = [a_n, b_n] (n \in \mathbb{N})$$, we know $$a_n \le b_n, \quad a_n \nearrow, \quad b_n \searrow$$.
We know

$$
\forall n, m \in \mathbb{N}, a_n \le a_{\max{(n,m)}} \le b_{\max_{(n,m)}} \le b_{m}
$$

In other words, for every $$m \in \mathbb{N}$$, $$b_m$$ is a upper bound of $$\{a_n \vert n \in \mathbb{N}\}$$.
Let $$c=\lim_{n\to\infty}a_n$$.
Then $$c$$ is the least uppber bound, $$c \ge a_n$$ for all $$n$$.
For all $$m$$, $$a_n \le b_m$$, take the limits $$\lim_{n\to\infty} a_n \le \lim_{n\to\infty} b_m$$, thus $$c \le b_m$$ for all $$m$$.

Ex2: (1) What if $$I_n = (a_n, b_n)$$ nested, but $$a_n \nearrow\nearrow$$ and $$b_n \searrow\searrow$$?

In this case the intersections are non-empty.

$$
\forall n, m \in \mathbb{N}, a_n < a_{\max(n,m)} < b_{\max(n,m)} < b_{m}
$$

Let $$c = \lim_{n\to\infty} a_n$$, then $$c$$ is the least uppber bound, $$c \ge a_{n+1} > a_{n}$$ for all $$n$$.
Also $$c \le b_{m+1} < b_m$$

(2) $$I_n = (a_n, \infty)$$, nested and $$\{a_n\}$$ bounded above.

In this case the intersections are non-empty. Let $$c$$ be an upper bound. For all $$n$$, $$c \ge a_{n}$$, thus $$c + 1 \ge a_{n} + 1 > a_n$$

## Equivalence

gapless is equivalent to Weierstrass, to $$(\text{ mono } + \text{ Archimedean })$$ to $$(\text{ nexted interval } + \text{ Archimedean })$$.

These expressions are used to determine if we can define something and it is a real number.
For example, if we can find a bounded increasing sequence, then we know there is a real number to be its limit.

## Cauchy Sequence

A sequence $$a_n (n \in \mathbb{N})$$ in $$\mathbb{R}$$ is a Cauchy sequence if

$$
\forall \varepsilon > 0\, \exists N \in \mathbb{N} \, [n, m \ge N \implies \vert a_n - a_m \vert < \varepsilon]
$$

It is easy to see

- convergent $$\implies$$ Cauchy

- Cauchy $$\implies$$ bounded

Theorem: Cauchy $$\iff$$ convergent.

To prove the theorem, we need the definition of upper and lower sequence.

## Upper And Lower Sequence

Definition:

For a bounded sequence $$a_n$$, let

$$
u_n = \sup \{a_m \vert m \ge n\}
$$

$$
l_n = \inf \{a_m \vert m \ge n\}
$$

we call $$u_n$$ the upper sequence of $$a_n$$, $$l_n$$ the lower sequence of $$a_n$$.
We want to show for the bounded sequence $$a_n$$, the upper sequence and lower sequence converge: $$\lim_{n\to\infty} u_n, \lim_{n\to\infty} l_n$$ exists.
It is easy to see $$u_n \searrow, \, l_n \nearrow$$.
Also $$l_n \le a_n \le u_n$$.

For example, to show $$u_n \searrow$$, we need to show $$\forall i \ge 1, u_{i+1} \le u_{i}$$.
Were this false, $$\exists i \ge 1, u_{i} < u_{i+1}$$.

$$
u_{i} < u_{i+1} = \sup \{a_m \vert m \ge i + 1\}
$$

$$
u_{i} \text{ is not upper bound of } \{a_m \vert m \ge i + 1\}
$$

$$
u_{i} \text{ is upper bound of } \{a_m \vert m \ge i\} \implies u_{i} \text{ is upper bound of } \{a_m \vert m \ge i+1\}
$$

Also, the sequence $$\{u_n\}$$, $$\{l_n\}$$ is bounded.
For example, to show $$\{u_n\}$$ is bounded, since $$u_n \searrow$$, we only need to show $$\{u_n\}$$ has lower bound.
Let $$A$$ be a lower bound of $$\{a_n\}$$, we want to show $$A$$ is also a lower bound of $$\{u_n\}$$. Were this false, $$A$$ is not a lower bound of $$\{u_n\}$$

$$
\exists i, u_i < A
$$

$$
\exists i, a_i \le \sup \{a_m \vert m \ge i\} = u_i < A
$$

Then we have $$a_i < A$$, this is impossible, since $$A$$ is lower bound of $$\{a_n\}$$.

$$
\overline{\lim_{n\to\infty}} a_{n}=\limsup_{n\to\infty} a_n := \lim_{n\to\infty} u_n
$$

$$
\underline{\lim}\limits_{n\to\infty} \liminf_{n\to\infty} a_n := \lim_{n\to\infty} l_n
$$

Ex4: $$a_n$$ converges $$\iff$$ $$\limsup_{n\to\infty} a_n = \liminf_{n\to\infty} a_n \ne \infty$$.

And if it is the case, $$\lim_{n\to\infty}a_n = \limsup_{n\to\infty} a_n = \limsup_{n\to\infty} a_n$$

We have $$ l_n \le a_n \le u_n $$

&nbsp; $$\Leftarrow$$ is from squeeze theorem.

&nbsp; $$\implies$$, Let $$\lim_{n\to\infty}a_n$$ = A

$$
\forall \epsilon > 0\, \exists N \in\mathbb{N}\, [n \ge N \implies A - \varepsilon < a_n < A + \varepsilon ]
$$

thus $$A - \varepsilon$$ is a lower bound of $$\{a_m \vert m \ge N\}$$, and $$l_N$$ is the greatest lower bound of $$\{a_m \vert m \ge N\}$$, thus $$A - \varepsilon \le l_N \le l_n$$ for all $$n \ge N$$. Similarly

$$
\forall \epsilon > 0\, \exists N \in\mathbb{N}\, [n \ge N \implies A - \varepsilon \le l_{N} \le l_n \le a_n \le u_n \le u_N \le A + \varepsilon ]
$$

thus $$\limsup_{n\to\infty} a_n = \liminf_{n\to\infty} a_n = A$$.
